ETCS_Mult.thy
@@ -489,7 +489,7 @@ proof(rule natural_number_object_func_unique[where f="successor", where X="\<nat
 qed
 
   show ?thesis
-    using assms cfunc_type_def comp_associative id3 id_left_unit2 mult2_type mult_apply1right s0b_id_type succ_n_type successor_type terminal_func_type zero_type by auto
+    using assms cfunc_type_def comp_associative id3 id_left_unit2 mult2_type mult_apply1right s0b_id_type succ_n_type successor_type terminal_func_type zero_type by smt
 qed
 
 
@@ -715,7 +715,7 @@ also have "... =
             (left_cart_proj (\<nat>\<^sub>c\<times>\<^sub>c \<nat>\<^sub>c) \<nat>\<^sub>c),(right_cart_proj (\<nat>\<^sub>c\<times>\<^sub>c \<nat>\<^sub>c) \<nat>\<^sub>c)\<rangle>\<rangle>)\<^sup>\<sharp> )) \<circ>\<^sub>c
             (id\<^sub>c (\<nat>\<^sub>c\<times>\<^sub>c \<nat>\<^sub>c) \<times>\<^sub>f zero) 
              \<circ>\<^sub>c x"
-    using cfunc_type_def comp_associative transpose_func_def x_type by (typecheck_cfuncs, auto)
+    using cfunc_type_def comp_associative transpose_func_def x_type by (typecheck_cfuncs, smt (verit))
   also have "... =  (eval_func \<nat>\<^sub>c (\<nat>\<^sub>c \<times>\<^sub>c \<nat>\<^sub>c) \<circ>\<^sub>c id\<^sub>c (\<nat>\<^sub>c \<times>\<^sub>c \<nat>\<^sub>c) \<times>\<^sub>f
           (add2 \<circ>\<^sub>c \<langle>mult2 \<circ>\<^sub>c \<langle>left_cart_proj \<nat>\<^sub>c \<nat>\<^sub>c \<circ>\<^sub>c left_cart_proj (\<nat>\<^sub>c \<times>\<^sub>c \<nat>\<^sub>c) \<nat>\<^sub>c,right_cart_proj (\<nat>\<^sub>c \<times>\<^sub>c \<nat>\<^sub>c) \<nat>\<^sub>c\<rangle>,
                   mult2 \<circ>\<^sub>c \<langle>right_cart_proj \<nat>\<^sub>c \<nat>\<^sub>c \<circ>\<^sub>c left_cart_proj (\<nat>\<^sub>c \<times>\<^sub>c \<nat>\<^sub>c) \<nat>\<^sub>c,right_cart_proj (\<nat>\<^sub>c \<times>\<^sub>c \<nat>\<^sub>c) \<nat>\<^sub>c\<rangle>\<rangle>)\<^sup>\<sharp> \<circ>\<^sub>c zero) \<circ>\<^sub>c \<langle>\<langle>p,q\<rangle>, id one\<rangle>"
@@ -856,7 +856,7 @@ also have "... = ((eval_func \<nat>\<^sub>c (\<nat>\<^sub>c\<times>\<^sub>c \<na
           also have "... = (add2 \<circ>\<^sub>c (add2 \<times>\<^sub>f (id\<^sub>c \<nat>\<^sub>c)) \<circ>\<^sub>c
           \<langle>(left_cart_proj (\<nat>\<^sub>c\<times>\<^sub>c\<nat>\<^sub>c) (\<nat>\<^sub>c\<^bsup>(\<nat>\<^sub>c\<times>\<^sub>c \<nat>\<^sub>c)\<^esup>)), eval_func \<nat>\<^sub>c (\<nat>\<^sub>c\<times>\<^sub>c \<nat>\<^sub>c)\<rangle>) 
         \<circ>\<^sub>c \<langle>id\<^sub>c (\<nat>\<^sub>c\<times>\<^sub>c \<nat>\<^sub>c)\<circ>\<^sub>c  \<langle>p,q\<rangle>, (mult2 \<circ>\<^sub>c (add2 \<times>\<^sub>f id\<^sub>c \<nat>\<^sub>c))\<^sup>\<sharp> \<circ>\<^sub>c r\<rangle>"
-            using cfunc_type_def comp_associative id_left_unit2 pq22idr_type pq_type by (typecheck_cfuncs, auto)
+            using cfunc_type_def comp_associative id_left_unit2 pq22idr_type pq_type by (typecheck_cfuncs, smt)
           also have "... =  ( (eval_func \<nat>\<^sub>c (\<nat>\<^sub>c\<times>\<^sub>c \<nat>\<^sub>c))\<circ>\<^sub>c 
                             (id\<^sub>c (\<nat>\<^sub>c\<times>\<^sub>c \<nat>\<^sub>c) \<times>\<^sub>f (add2 \<circ>\<^sub>c (add2 \<times>\<^sub>f (id\<^sub>c \<nat>\<^sub>c)) \<circ>\<^sub>c
                   \<langle>(left_cart_proj (\<nat>\<^sub>c\<times>\<^sub>c\<nat>\<^sub>c) (\<nat>\<^sub>c\<^bsup>(\<nat>\<^sub>c\<times>\<^sub>c \<nat>\<^sub>c)\<^esup>)), eval_func \<nat>\<^sub>c (\<nat>\<^sub>c\<times>\<^sub>c \<nat>\<^sub>c)\<rangle>)\<^sup>\<sharp>))\<circ>\<^sub>c \<langle>id\<^sub>c (\<nat>\<^sub>c\<times>\<^sub>c \<nat>\<^sub>c)\<circ>\<^sub>c  \<langle>p,q\<rangle>, (mult2 \<circ>\<^sub>c (add2 \<times>\<^sub>f id\<^sub>c \<nat>\<^sub>c))\<^sup>\<sharp> \<circ>\<^sub>c r\<rangle>"
@@ -1393,7 +1393,7 @@ proof -
             using comp_associative2 x_type by (typecheck_cfuncs, auto)
           also have "... = (eval_func \<nat>\<^sub>c \<nat>\<^sub>c \<circ>\<^sub>c (id\<^sub>c \<nat>\<^sub>c \<times>\<^sub>f (add2 \<circ>\<^sub>c \<langle>left_cart_proj \<nat>\<^sub>c (\<nat>\<^sub>c\<^bsup>\<nat>\<^sub>c\<^esup>),eval_func \<nat>\<^sub>c \<nat>\<^sub>c\<rangle>)\<^sup>\<sharp>) \<circ>\<^sub>c(id\<^sub>c \<nat>\<^sub>c \<times>\<^sub>f  (mult2 \<circ>\<^sub>c \<langle>right_cart_proj \<nat>\<^sub>c \<nat>\<^sub>c,left_cart_proj \<nat>\<^sub>c \<nat>\<^sub>c\<rangle>)\<^sup>\<sharp>)) \<circ>\<^sub>c x"
             using \<open>(add2 \<circ>\<^sub>c \<langle>left_cart_proj \<nat>\<^sub>c (\<nat>\<^sub>c\<^bsup>\<nat>\<^sub>c\<^esup>),eval_func \<nat>\<^sub>c \<nat>\<^sub>c\<rangle> \<circ>\<^sub>c id\<^sub>c \<nat>\<^sub>c \<times>\<^sub>f (mult2 \<circ>\<^sub>c \<langle>right_cart_proj \<nat>\<^sub>c \<nat>\<^sub>c,left_cart_proj \<nat>\<^sub>c \<nat>\<^sub>c\<rangle>)\<^sup>\<sharp>) \<circ>\<^sub>c x = add2 \<circ>\<^sub>c \<langle>left_cart_proj \<nat>\<^sub>c (\<nat>\<^sub>c\<^bsup>\<nat>\<^sub>c\<^esup>),eval_func \<nat>\<^sub>c \<nat>\<^sub>c\<rangle> \<circ>\<^sub>c (id\<^sub>c \<nat>\<^sub>c \<times>\<^sub>f (mult2 \<circ>\<^sub>c \<langle>right_cart_proj \<nat>\<^sub>c \<nat>\<^sub>c,left_cart_proj \<nat>\<^sub>c \<nat>\<^sub>c\<rangle>)\<^sup>\<sharp>) \<circ>\<^sub>c x\<close>
-            cfunc_type_def comp_associative transpose_func_def by (typecheck_cfuncs, auto)
+            cfunc_type_def comp_associative transpose_func_def by (typecheck_cfuncs, smt)
           also have "... = (eval_func \<nat>\<^sub>c \<nat>\<^sub>c \<circ>\<^sub>c id\<^sub>c \<nat>\<^sub>c \<times>\<^sub>f (add2 \<circ>\<^sub>c \<langle>left_cart_proj \<nat>\<^sub>c (\<nat>\<^sub>c\<^bsup>\<nat>\<^sub>c\<^esup>),eval_func \<nat>\<^sub>c \<nat>\<^sub>c\<rangle>)\<^sup>\<sharp> \<circ>\<^sub>c (mult2 \<circ>\<^sub>c \<langle>right_cart_proj \<nat>\<^sub>c \<nat>\<^sub>c,left_cart_proj \<nat>\<^sub>c \<nat>\<^sub>c\<rangle>)\<^sup>\<sharp>) \<circ>\<^sub>c x"
             by (typecheck_cfuncs,  simp add: identity_distributes_across_composition)
           then show "(eval_func \<nat>\<^sub>c \<nat>\<^sub>c \<circ>\<^sub>c id\<^sub>c \<nat>\<^sub>c \<times>\<^sub>f (mult2 \<circ>\<^sub>c \<langle>right_cart_proj \<nat>\<^sub>c \<nat>\<^sub>c,left_cart_proj \<nat>\<^sub>c \<nat>\<^sub>c\<rangle>)\<^sup>\<sharp> \<circ>\<^sub>c successor) \<circ>\<^sub>c x =
@@ -1718,7 +1718,7 @@ proof -
            also have "... = mult2 \<circ>\<^sub>c \<langle>mult2 \<circ>\<^sub>c y,id\<^sub>c \<nat>\<^sub>c \<circ>\<^sub>c (successor \<circ>\<^sub>c  r)\<rangle>"
              by (typecheck_cfuncs, smt cfunc_cross_prod_comp_cfunc_prod x_def)
            also have "... = mult2 \<circ>\<^sub>c \<langle>p \<cdot>\<^sub>\<nat> q, successor \<circ>\<^sub>c  r\<rangle>"
-             using cfunc_type_def comp_associative id_domain id_left_unit2 mult_def successor_type x_def y_def by auto
+             using cfunc_type_def comp_associative id_domain id_left_unit2 mult_def successor_type x_def y_def by smt
            also have "... = (p \<cdot>\<^sub>\<nat> q) \<cdot>\<^sub>\<nat> (successor \<circ>\<^sub>c  r)"
              by (simp add: mult_def)
            also have "... = (p \<cdot>\<^sub>\<nat> q) +\<^sub>\<nat> ((p \<cdot>\<^sub>\<nat> q)\<cdot>\<^sub>\<nat> r)"
@@ -1913,7 +1913,7 @@ eval_func \<nat>\<^sub>c (\<nat>\<^sub>c\<times>\<^sub>c\<nat>\<^sub>c)
     \<nat>\<^sub>c,\<langle>right_cart_proj \<nat>\<^sub>c \<nat>\<^sub>c \<circ>\<^sub>c
          left_cart_proj (\<nat>\<^sub>c \<times>\<^sub>c \<nat>\<^sub>c) \<nat>\<^sub>c,right_cart_proj (\<nat>\<^sub>c \<times>\<^sub>c \<nat>\<^sub>c) \<nat>\<^sub>c\<rangle>\<rangle> \<circ>\<^sub>c
   x\<rangle>"
-      using cfunc_type_def comp_associative id_left_unit2 x_def y_def by (typecheck_cfuncs, auto)
+      using cfunc_type_def comp_associative id_left_unit2 x_def y_def by (typecheck_cfuncs, smt)
 
 
 also have "... = add2 \<circ>\<^sub>c \<langle>mult2 \<circ>\<^sub>c (id (\<nat>\<^sub>c \<times>\<^sub>c \<nat>\<^sub>c)  \<circ>\<^sub>c  left_cart_proj (\<nat>\<^sub>c\<times>\<^sub>c \<nat>\<^sub>c) \<nat>\<^sub>c) , 
